proof/Ax.v
@@ -94,9 +94,15 @@ Lemma let_reduction_spec: forall x e_x e (v: value),
     tlete x e_x e -->* v <-> (exists (v_x: value), e_x -->* v_x /\ (subst x v_x e) -->* v).
 Admitted.
 
+Lemma letapp_reduction_spec: forall x (f: value) (v1 : value) (v : value) e,
+    tletapp x f v1 e -->* v <->
+    (exists x_m T_m e_m,
+        f = vlam x_m T_m e_m /\ (tlete x (subst x_m v1 e_m) e) -->* v).
+Admitted.
+
 Lemma reduction_eq_implies_ty_eq: forall e1 e2,
-    (forall (v: value), e1 -->* v <-> e2 -->* v) ->
-    (forall Gamma T, Gamma \N- e1 \Tin T <-> Gamma \N- e2 \Tin T).
+    (forall (v: value), e1 -->* v -> e2 -->* v) ->
+    (forall Gamma T, Gamma \N- e1 \Tin T -> Gamma \N- e2 \Tin T).
 Admitted.
 
 Lemma reduction_eq_implies_eq: forall e1 e2,
@@ -104,8 +110,17 @@ Lemma reduction_eq_implies_eq: forall e1 e2,
 Proof with eauto.
   intros.
   split.
-  - split. intros... rewrite <- H... apply reduction_eq_implies_ty_eq... symmetry...
-  - split. intros... rewrite H... apply reduction_eq_implies_ty_eq...
+  - split. intros... rewrite <- H... apply reduction_eq_implies_ty_eq... intros... rewrite <- H...
+  - split. intros... rewrite H... apply reduction_eq_implies_ty_eq... intros... rewrite H...
+Qed.
+
+Lemma reduction_sub_implies_sub: forall e1 e2,
+    (forall (v: value), e1 -->* v -> e2 -->* v) -> e1 <-< e2.
+Proof with eauto.
+  intros.
+  split.
+  - intros...
+  - intros... eapply reduction_eq_implies_ty_eq...
 Qed.
 
 Lemma subst_letx_same: forall x1 v1 x,
@@ -131,6 +146,14 @@ Proof with eauto.
   - exists v. split...
 Qed.
 
+Lemma reduce_value_prop_same_post: forall (v: value) P,
+   (exists (v_x : value), P v_x /\ v_x -->* v) <-> P v.
+Proof with eauto.
+  split; intros.
+  - setoid_rewrite value_only_reduce_to_itself in H. destruct H as (v' & Hv' & HH); subst...
+  - exists v. split...
+Qed.
+
 Lemma eta_app_value_value: forall x (v1 v2: value) x1 x2,
     x1 <> x2 -> ~ x1 \FVtm v2 ->
     tletapp x v1 v2 x <=< tlete x1 v1 (tlete x2 v2 (tletapp x x1 x2 x)).
@@ -144,9 +167,9 @@ Proof with eauto.
     destruct (eqb_spec x2 x); destruct (eqb_spec x1 x); simpl; subst...
     + rewrite <- eqb_neq in n... rewrite n...
     + rewrite <- eqb_neq in n... rewrite n...
-  - rewrite let_reduction_spec in HE. apply reduce_value_prop_same in HE.
+  - rewrite let_reduction_spec in HE. rewrite reduce_value_prop_same in HE.
     simpl in HE. rewrite not_free_rewrite_value in HE... rewrite <- eqb_neq in H. rewrite H in HE. rewrite eqb_refl in HE.
-    rewrite let_reduction_spec in HE. apply reduce_value_prop_same in HE.
+    rewrite let_reduction_spec in HE. rewrite reduce_value_prop_same in HE.
     simpl in HE. rewrite not_free_rewrite_value in HE... rewrite eqb_refl in HE.
     destruct (eqb_spec x2 x); destruct (eqb_spec x1 x); simpl in HE; subst...
     + rewrite <- eqb_neq in n... rewrite n in HE...
@@ -172,77 +195,264 @@ Admitted.
 Lemma eta_reduction: forall x1 (f: value) x2 (v: value),
     ~ x1 \FVvalue v ->
     (tletapp x2 f v x2) <=< (tlete x1 f (tletapp x2 x1 v x2)).
-Admitted.
+Proof with eauto.
+    intros. apply reduction_eq_implies_eq.
+    split. intro HE.
+    - rewrite let_reduction_spec. rewrite reduce_value_prop_same.
+      simpl. rewrite not_free_rewrite_value...
+      rewrite eqb_refl.
+      destruct (eqb_spec x1 x2); simpl. apply HE. apply HE.
+    - rewrite let_reduction_spec. rewrite reduce_value_prop_same.
+      simpl. rewrite not_free_rewrite_value...
+      rewrite eqb_refl.
+      destruct (eqb_spec x1 x2); simpl. intro HE. apply HE. intro HE. apply HE.
+ Qed.
+
+Ltac lete_eta_step := rewrite let_reduction_spec; simpl;
+                      try (rewrite reduce_value_prop_same; simpl);
+                      try (rewrite reduce_value_prop_same_post; simpl);
+                      try (rewrite not_free_rewrite_value; simpl);
+                      try rewrite eqb_refl; try rewrite eqb_neq.
+
+Ltac lete_eta_step_in H := rewrite let_reduction_spec in H; simpl in H;
+                           try (rewrite reduce_value_prop_same in H; simpl);
+                           try (rewrite reduce_value_prop_same_post in H; simpl);
+                           try (rewrite reduce_value_prop_same in H; simpl in H);
+                           try rewrite not_free_rewrite_value in H;
+                           try rewrite eqb_refl in H; try rewrite eqb_neq in H.
+
+Lemma reduce_letapp_value_prop_same: forall (v: value) P,
+   (exists (v_x : value), v -->* v_x /\ P v_x) <-> P v.
+Proof with eauto.
+  split; intros.
+  - setoid_rewrite value_only_reduce_to_itself in H. destruct H as (v' & Hv' & HH); subst...
+  - exists v. split...
+Qed.
+
+Lemma tail_lete: forall x e (v: value), tlete x e x -->* v <-> e -->* v.
+Proof with eauto.
+  intros. split; intro HE.
+  - lete_eta_step_in HE. destruct HE as (v_x & HEv_x & Hvv). rewrite value_only_reduce_to_itself in Hvv; subst...
+  - lete_eta_step. exists v. split...
+Qed.
+
+Ltac letapp_eta_step Hletapp := rewrite letapp_reduction_spec; intro Hletapp;
+                                destruct Hletapp as (x_m & T_m & e_m & Happ1 & Happ2); inversion Happ1; subst; clear Happ1;
+                                try (lete_eta_step_in Happ2; rewrite reduce_value_prop_same_post in Happ2).
 
 Lemma eta_application_const_to_lete_const: forall x2 x T e (c_x: constant),
     (tlete x c_x e) <=< (tletapp x2 (vlam x T e) c_x x2).
-Admitted.
+Proof with eauto.
+    intros. apply reduction_eq_implies_eq.
+    split. intro HE.
+    - lete_eta_step_in HE.
+      rewrite letapp_reduction_spec. exists x, T, e. split... rewrite tail_lete...
+    - lete_eta_step. letapp_eta_step Hletapp...
+ Qed.
 
 Lemma eta_lete_const_to_subst: forall x e (c_x: constant),
     (subst x c_x e) <=< (tlete x c_x e).
+Proof with eauto.
+    intros. apply reduction_eq_implies_eq.
+    split. intro HE.
+    - rewrite let_reduction_spec. rewrite reduce_value_prop_same. apply HE.
+    - rewrite let_reduction_spec. rewrite reduce_value_prop_same.  trivial.
+Qed.
+
+Lemma eta_in_lam: forall a T e1 e2,
+    (forall (v: value), e1 -->* v -> e2 -->* v) <-> (forall (v: value), vlam a T e1 -->* v -> vlam a T e2 -->* v).
 Admitted.
 
 Lemma eta_lete_const_to_subst_in_lam: forall a T x e (c_x: constant),
     (vlam a T (subst x c_x e)) <=< (vlam a T (tlete x c_x e)).
-Admitted.
+Proof with eauto.
+  intros. apply reduction_eq_implies_eq.
+  split.
+  - apply eta_in_lam. intros v' HE. lete_eta_step...
+  - apply eta_in_lam. intros v' HE. lete_eta_step_in HE...
+Qed.
 
 Lemma eta_closed_term_can_captured_by_lam: forall a e_a Ta x T e,
     empty \N- e_a \Tin Ta -> a <> x ->
     (vlam x T (tlete a e_a e)) <=< (tlete a e_a (vlam x T e)).
+Proof with eauto.
 Admitted.
 
 Lemma eta_matchb_true: forall e1 e2, e1 <=< (tmatchb true e1 e2).
-Admitted.
+Proof with auto.
+  intros. apply reduction_eq_implies_eq.
+  split.
+  - intros. econstructor...
+  - intros. inversion H; subst... inversion H0; subst...
+Qed.
 
 Lemma eta_matchb_false: forall e1 e2, e2 <=< (tmatchb false e1 e2).
-Admitted.
+Proof with auto.
+  intros. apply reduction_eq_implies_eq.
+  split.
+  - intros. econstructor...
+  - intros. inversion H; subst... inversion H0; subst...
+Qed.
 
 Lemma eta1: forall x1 x T e x2 (c_x:constant) x0,
     x1<> x2 -> ~ x1 \FVtm c_x ->
     (tlete x1 (vlam x T e) (tlete x2 c_x (tletapp x0 x1 x2 x0))) <=< (tlete x c_x e).
+Proof with eauto.
+    intros. apply reduction_eq_implies_eq.
+    split. intro HE.
+    - lete_eta_step_in HE.
+      lete_eta_step.
+      destruct (eqb_spec x1 x2); destruct (eqb_spec x1 x0); simpl in HE; subst...
+      + exfalso...
+      + exfalso...
+      + lete_eta_step_in HE. rewrite letapp_reduction_spec in HE.
 Admitted.
 
 Lemma eta11: forall x e_x e x1 x2 x0 T1 T2,
     ~ x1 \FVtm e_x ->
     (tlete x e_x e) <-< tlete x1 (vlam x (T1 t--> T2) e) (tlete x2 e_x (tletapp x0 x1 x2 x0)).
+Proof with eauto.
+  intros. apply reduction_sub_implies_sub.
+  intros v HE.
+  lete_eta_step. lete_eta_step.
+  lete_eta_step_in HE. destruct HE as (v_x & HE1 & HE2).
+  exists v_x. split...
+  - assert ([x1 := vlam x (T1 t--> T2) e] e_x = e_x) as He_x... rewrite He_x...
+  -
 Admitted.
 
 Lemma eta2: forall e2 (c2: constant) x1 e1 x2 x,
     e2 -->* c2 ->
     (tlete x1 e1 (tlete x2 c2 (tletapp x x1 x2 x))) <-< (tlete x1 e1 (tlete x2 e2 (tletapp x x1 x2 x))).
-Admitted.
+Proof with eauto.
+  intros. apply reduction_sub_implies_sub.
+  intros v HE.
+  lete_eta_step_in HE. lete_eta_step.
+  destruct HE as (v_x & HE1 & HE2). exists v_x. split...
+  lete_eta_step_in HE2. lete_eta_step...
+  exists c2. split... assert ([x1 := v_x] e2 = e2)... rewrite H0...
+Qed.
 
 Lemma eta3: forall x1 a (e_a: tm) Ta e1 x2 e2 x,
     empty \N- e_a \Tin Ta ->
     (tlete a e_a (tlete x1 e1 (tlete x2 e2 (tletapp x x1 x2 x))))
       <=< (tlete x1 (tlete a e_a e1) (tlete x2 (tlete a e_a e2) (tletapp x x1 x2 x))).
+Proof with eauto.
+  intros. apply reduction_eq_implies_eq.
+  split. intro HE.
+  - lete_eta_step_in HE.
+    destruct HE as (v_a & HE1 & HE).
+    lete_eta_step_in HE. destruct HE as (v1 & HE2 & HE).
+    lete_eta_step... exists v1... split... lete_eta_step... lete_eta_step...
+    destruct (eqb_spec a x1); subst...
+    + simpl in HE. lete_eta_step_in HE...
+      destruct HE as (v2 & HEv2 & HE). exists v2. split... lete_eta_step. exists v1. split...
 Admitted.
 
-Lemma eta_subst_in_const: forall a e_x (c: constant), (tlete a e_x c) <=< c.
+(* Lemma eta_subst_in_const: forall a (e_x: constant) (c: constant), c <-< (tlete a e_x c). *)
+(* Proof with eauto. *)
+(*   intros. apply reduction_sub_implies_sub. *)
+(*   intros v HE. *)
+(*   lete_eta_step... *)
+(* Qed. *)
+
+Lemma eta_subst_in_const: forall a (e_x: tm) (v_x: constant) (c: constant),
+    c <-< (tlete a e_x c).
+Proof with eauto.
 Admitted.
 
 Lemma eta_snd_let_reduce: forall x1 e1 x2 e2 x (c2: constant),
     e2 -->* c2 ->
     (tlete x1 e1 (tlete x2 c2 (tletapp x x1 x2 x))) <-< (tlete x1 e1 (tlete x2 e2 (tletapp x x1 x2 x))).
-Admitted.
+Proof with eauto.
+  intros. apply reduction_sub_implies_sub.
+  intros v HE.
+  lete_eta_step_in HE. destruct HE as (v1 & H1 & HE)...
+  lete_eta_step_in HE.
+  lete_eta_step. exists v1. split... lete_eta_step. exists c2. split... rewrite not_free_rewrite...
+Qed.
 
 Lemma eta4: forall x1 (v1: value) x2 (c2: constant) x,
     x1 <> x2 ->
     tlete x1 v1 (tlete x2 c2 (tletapp x x1 x2 x)) <-< tletapp x v1 c2 x.
+Proof with eauto.
+  intros. apply reduction_sub_implies_sub.
+  intros v HE.
+  lete_eta_step_in HE. lete_eta_step_in HE.
+  destruct (eqb_spec x1 x2); subst; simpl in HE; simpl...
+  - exfalso...
+  - rewrite eqb_refl in HE. rewrite not_free_rewrite_value in HE...
+    destruct (eqb_spec x2 x); subst; simpl in HE; simpl...
+    + destruct (eqb_spec x1 x); subst; simpl in HE; simpl...
+    + destruct (eqb_spec x1 x); subst; simpl in HE; simpl...
+      destruct (eqb_spec x2 x); subst; simpl in HE; simpl... exfalso...
+      destruct (eqb_spec x2 x); subst; simpl in HE; simpl... exfalso...
+Qed.
+
+Lemma subst_var_value: forall x v1, [x := x ]v v1 = v1.
+Admitted.
+
+Lemma subst_var: forall x v1, [x := x ] v1 = v1.
 Admitted.
 
 Lemma eta5: forall x1 (v1: value) x2 (id2: string) x,
     x1 <> x2 -> ~ x1 \FVvalue id2 ->
     (tlete x1 v1 (tlete x2 id2 (tletapp x x1 x2 x))) <-< tletapp x v1 id2 x.
-Admitted.
+Proof with eauto.
+  intros. apply reduction_sub_implies_sub.
+  intros v HE.
+  lete_eta_step_in HE. lete_eta_step_in HE.
+  destruct (eqb_spec x1 id2); subst; simpl in HE; simpl...
+  - exfalso... apply H0... constructor...
+  - destruct (eqb_spec x1 x2); subst; simpl in HE; simpl... exfalso...
+    destruct (eqb_spec x2 id2); subst; simpl in HE; simpl; try rewrite eqb_refl in HE; try rewrite eqb_neq in HE...
+    + rewrite subst_var_value in HE.
+      destruct (eqb_spec id2 x); subst; simpl in HE; simpl; try rewrite eqb_refl in HE; try rewrite eqb_neq in HE...
+      destruct (eqb_spec x1 x); subst; simpl in HE; simpl; try rewrite eqb_refl in HE; try rewrite eqb_neq in HE...
+      rewrite subst_var in HE.
+      destruct (eqb_spec x1 x); subst; simpl in HE; simpl...
+    + rewrite not_free_rewrite_value in HE...
+      destruct (eqb_spec x2 x); subst; simpl in HE; simpl...
+      destruct (eqb_spec x1 x); subst; simpl in HE; simpl...
+      destruct (eqb_spec x1 x); subst; simpl in HE; simpl...
+      destruct (eqb_spec x2 x); subst; simpl in HE; simpl... exfalso...
+      destruct (eqb_spec x2 x); subst; simpl in HE; simpl... exfalso...
+Qed.
 
 Lemma eta6: forall x1 (v1 v2: value) x2 x,
-    ~ x1 \FVvalue v2 ->
+    ~ x1 \FVvalue v2 -> x1 <> x2 ->
     tlete x1 v1 (tlete x2 v2 (tletapp x x1 x2 x)) <-< tletapp x v1 v2 x.
-Admitted.
+Proof with eauto.
+  intros. apply reduction_sub_implies_sub.
+  intros v HE.
+  lete_eta_step_in HE... lete_eta_step_in HE...
+  destruct (eqb_spec x1 x2); subst; simpl in HE; simpl; try rewrite eqb_refl in HE; try rewrite eqb_neq in HE... exfalso...
+  - rewrite not_free_rewrite_value in HE...
+    destruct (eqb_spec x2 x); subst; simpl in HE; simpl; try rewrite eqb_refl in HE; try rewrite eqb_neq in HE...
+    + destruct (eqb_spec x1 x); subst; simpl in HE; simpl; try rewrite eqb_refl in HE; try rewrite eqb_neq in HE...
+    + destruct (eqb_spec x2 x); subst; simpl in HE; simpl; try rewrite eqb_refl in HE; try rewrite eqb_neq in HE... exfalso...
+      destruct (eqb_spec x1 x); subst; simpl in HE; simpl; try rewrite eqb_refl in HE; try rewrite eqb_neq in HE...
+      destruct (eqb_spec x2 x); subst; simpl in HE; simpl; try rewrite eqb_refl in HE; try rewrite eqb_neq in HE... exfalso...
+      destruct (eqb_spec x2 x); subst; simpl in HE; simpl; try rewrite eqb_refl in HE; try rewrite eqb_neq in HE... exfalso...
+Qed.
+
+Ltac super_eqb_spec x1 x HE :=
+  destruct (eqb_spec x1 x); subst; simpl in HE; simpl; try rewrite eqb_refl in HE; try rewrite eqb_neq in HE; eauto.
 
 Lemma eta7: forall x v1 v2 e, (tlete x (tletapp x v1 v2 x) e) <=< (tletapp x v1 v2 e).
-Admitted.
+Proof with eauto.
+    intros. apply reduction_eq_implies_eq.
+    split; intro HE.
+    - lete_eta_step_in HE... destruct HE as (v_x & Hv_x & HH).
+      rewrite letapp_reduction_spec in Hv_x. destruct Hv_x as (x_m & T_m & e_m & H1 & H2); subst...
+      rewrite letapp_reduction_spec. exists x_m, T_m, e_m. split... lete_eta_step_in H2...
+      destruct H2 as (v_m & Hv_m & Hvm2). lete_eta_step... exists v_x. split... eapply multi_trans...
+    - rewrite letapp_reduction_spec in HE. destruct HE as (x_m & T_m & e_m & H1 & H2); subst...
+      lete_eta_step_in H2... destruct H2 as (v_m & Hv_m & Hvm2).
+      lete_eta_step... exists v_m. split... rewrite letapp_reduction_spec.
+      exists x_m, T_m, e_m. split... lete_eta_step. exists v_m. split...
+Qed.
+
 
 Lemma eta8: forall x op v1 v2 e, (tlete x (tletbiop x op v1 v2 x) e) <=< (tletbiop x op v1 v2 e).
 Admitted.
@@ -266,15 +476,36 @@ Lemma eta_drop_lete_not_bot: forall x e_x0 e,
     (exists c0 : constant, e_x0 -->* c0) ->
     ~ x \FVtm e ->
     (tlete x e_x0 e) <=< e.
-Admitted.
+Proof with eauto.
+    intros. apply reduction_eq_implies_eq.
+    split; intro HE.
+    - lete_eta_step_in HE... destruct HE as (v_x & Hv_x & HH). rewrite not_free_rewrite in HH...
+    - lete_eta_step. destruct H as (v_x & Hv_x). exists v_x. split... rewrite not_free_rewrite...
+Qed.
+
 
 Lemma eta_lete_neq: forall x a c_x e_x e,
     a <> x ->
     tlete x (tlete a c_x e_x) (tlete a c_x e) <-< tlete a c_x (tlete x e_x e).
-Admitted.
+Proof with eauto.
+  intros. apply reduction_sub_implies_sub.
+  intros v HE.
+  lete_eta_step_in HE...
+  destruct HE as (v_x & Hv_x & HE). rewrite not_free_rewrite in HE...
+  super_eqb_spec x a HE. exfalso...
+  - lete_eta_step_in HE... destruct HE as (v' & Hv' & HE). lete_eta_step. exists v'. split...
+    lete_eta_step_in Hv_x... rewrite not_free_rewrite...
+    destruct Hv_x as (vx' & Hvx' & Hv_x). rewrite not_free_rewrite in Hv_x... lete_eta_step. exists v_x. split...
+    super_eqb_spec a x HE. exfalso...
+    rewrite not_free_rewrite... rewrite not_free_rewrite in HE... rewrite not_free_rewrite in HE...
+    rewrite not_free_rewrite...
+Qed.
 
 Lemma eta_fix1: forall x1 f (T: base_ty) tau x e x2 (c_x': constant) x0,
     (tletapp x (vfix f (T t--> tau) x T e) c_x' x) <-< (tlete x1 (vfix f (T t--> tau) x T e) (tlete x2 c_x' (tletapp x0 x1 x2 x0))).
+Proof with eauto.
+  intros. apply reduction_sub_implies_sub.
+  intros v HE.
 Admitted.
 
 Lemma eta_fix2: forall x1 f (T: base_ty) tau x e x2 (c_x: constant),
@@ -290,7 +521,19 @@ Admitted.
 
 Lemma eta_fix4: forall a f (Tx: base_ty) tau x e (c_x: constant),
     tlete a c_x (vlam x Tx (vlam f (Tx t--> tau) e)) <-< vlam x Tx (vlam f (Tx t--> tau) (tlete a c_x e)).
-Admitted.
+Proof with eauto.
+  intros. apply reduction_sub_implies_sub.
+  intros v HE.
+  lete_eta_step_in HE...
+  generalize dependent v. rewrite <- eta_in_lam.
+  intros v HE.
+  super_eqb_spec a x HE.
+  - generalize dependent v. rewrite <- eta_in_lam. intros v HE.
+    lete_eta_step. rewrite not_free_rewrite...
+  - generalize dependent v. rewrite <- eta_in_lam. intros v HE.
+    super_eqb_spec a f HE.
+    lete_eta_step. rewrite not_free_rewrite...
+Qed.
 
 Lemma eta_fix5: forall a f (Tx: base_ty) tau x e (c_x: constant),
     vfix f (Tx t--> tau) x Tx (tlete a c_x e) <-< tlete a c_x (vfix f (Tx t--> tau) x Tx e).
@@ -298,7 +541,18 @@ Admitted.
 
 Lemma eta_fix6: forall a f (Tx: base_ty) tau x e e_x,
     tlete a e_x (vlam x Tx (vlam f (Tx t--> tau) e)) <-< vlam x Tx (vlam f (Tx t--> tau) (tlete a e_x e)).
-Admitted.
+Proof with eauto.
+  intros. apply reduction_sub_implies_sub.
+  intros v HE.
+  lete_eta_step_in HE... destruct HE as (v_x & Hv_x & HE).
+  generalize dependent v. rewrite <- eta_in_lam. intros v HE.
+  super_eqb_spec a x HE.
+  - generalize dependent v. rewrite <- eta_in_lam. intros v HE.
+    lete_eta_step. exists v_x. split... rewrite not_free_rewrite...
+  - generalize dependent v. rewrite <- eta_in_lam. intros v HE.
+    super_eqb_spec a f HE. lete_eta_step. exists v_x. split... rewrite not_free_rewrite...
+    lete_eta_step. exists v_x. split...
+Qed.
 
 Lemma eta_fix7: forall a f (Tx: base_ty) tau x e (e_x: tm),
     vfix f (Tx t--> tau) x Tx (tlete a e_x e) <-< tlete a e_x (vfix f (Tx t--> tau) x Tx e).
@@ -307,7 +561,13 @@ Admitted.
 Lemma eta_self1: forall x1 e e' x2 (c_x: tm) x,
     e <-< e' ->
     tlete x1 e (tlete x2 c_x (tletapp x x1 x2 x)) <-< tlete x1 e' (tlete x2 c_x (tletapp x x1 x2 x)).
-Admitted.
+Proof with eauto.
+  intros. apply reduction_sub_implies_sub.
+  intros v HE. destruct H as (HEE & HEE').
+  lete_eta_step_in HE... destruct HE as (v' & Hv' & HE). apply HEE in Hv'.
+  lete_eta_step. exists v'. split...
+Qed.
+
 
 Lemma eta_op_reducetion: forall op c_a c_b c_res x x0 x1 x2 x3 x4,
     eval_op op c_a c_b c_res ->
@@ -317,18 +577,37 @@ Admitted.
 Lemma eta_self2: forall x c_x e e',
     e <-< e' ->
     tlete x c_x e <-< tlete x c_x e'.
-Admitted.
+Proof with eauto.
+  intros. apply reduction_sub_implies_sub.
+  intros v HE. destruct H as (HEE & HEE').
+  lete_eta_step_in HE... destruct HE as (vc & Hv' & HE). rewrite not_free_rewrite in HE...
+  lete_eta_step. exists vc. split... rewrite not_free_rewrite...
+Qed.
 
 Lemma eta_a3: forall id (c_x: constant) e1 e2,
   tlete id c_x (tmatchb c_x e1 e2) <-< tlete id c_x (tmatchb id e1 e2).
-Admitted.
+Proof with eauto.
+  intros. apply reduction_sub_implies_sub.
+  intros v HE.
+  lete_eta_step_in HE... rewrite not_free_rewrite in HE... rewrite not_free_rewrite in HE...
+  lete_eta_step. rewrite not_free_rewrite... rewrite not_free_rewrite...
+Qed.
 
 Lemma eta_a4: forall id a (c_x: tm),
     id <> a -> tlete a c_x id <-< id.
-Admitted.
+Proof with eauto.
+  intros. apply reduction_sub_implies_sub.
+  intros v HE.
+  lete_eta_step_in HE... destruct HE as (v' & Hv' & HE).
+  super_eqb_spec a id HE. exfalso...
+Qed.
 
 Lemma eta_match1: forall a c_x (c: constant) e1 e2,
     tlete a c_x (tmatchb c e1 e2) <-< tmatchb c (tlete a c_x e1) (tlete a c_x e2).
+Proof with eauto.
+  intros. apply reduction_sub_implies_sub.
+  intros v HE.
+  lete_eta_step_in HE... destruct HE as (v' & Hv' & HE). rewrite not_free_rewrite in HE... rewrite not_free_rewrite in HE...
 Admitted.
 
 Lemma eta_match2: forall (a id: string) (c_x: tm) e1 e2,
@@ -338,7 +617,18 @@ Admitted.
 
 Lemma eta_match3: forall (id: string) (c: constant) (e_x: tm) e1 e2,
     tlete id e_x (tmatchb c e1 e2) <-< tlete id e_x (tmatchb id e1 e2).
+Proof with eauto.
+  intros. apply reduction_sub_implies_sub.
+  intros v HE.
+  lete_eta_step_in HE... destruct HE as (v' & Hv' & HE).
+  lete_eta_step. exists v'.
 Admitted.
 
+
 Lemma eta_a2: forall id c_x, tlete id c_x id <-< c_x.
-Admitted.
+Proof with eauto.
+  intros. apply reduction_sub_implies_sub.
+  intros v HE.
+  lete_eta_step_in HE... destruct HE as (v' & Hv' & HE).
+  eapply multi_trans...
+Qed.
